extract/oracles.ml
@@ -1,7 +1,7 @@
 (* Required since the termination of the `Vm.run` function cannot be proved *)
 let fuel_vm = 1000;;
 
-(* Required since we don't provide a proof of the liveness analysis algorithm *)
+(* Required since we don't include a proof for the termination of the liveness analysis algorithm *)
 let fuel_analyze = 50;;
 
 (* Required since we don't include the proof for the termination of the SSA destruction algorithm *)
